refactoring + fixed other errors

Main.fst
@@ -3,35 +3,55 @@ module Main
 open FStar.List.Tot.Base
 open FStar.String
 open FStar.IO
-open Utils
 open FormulaT
+open Cnf
+// open Tseitin
 
 
-let rec list_int_to_list_string (a:list int) : list string
-   = match a with
-      | [] -> []
-      | hd::tl -> string_of_int hd :: (list_int_to_list_string tl)
 
- let main = //let f0 = Var 0 in
-//            let f1 = Var 1 in
-//            let f2 = Var 2 in
-//            let f3 = Var 3 in 
-         //   let var_for_rule_0 = DImplies f0 f1 in
-         //   let var_for_rule_1 = Implies f0 f1 in
-         //   let var_for_rule_2 = Or f0 (And f1 f2) in
-         //   let var_for_rule_3 = Or (And f1 f2) (DImplies f0 f1) in
-         //   let var_for_rule_5 = Or f0 (Or f1 f2) in
-         //   let var_for_rule_6 = And f0 (And f1 f2) in
-         //   let var_for_rule_7 = Not (And f0 f1) in
-         //   let var_for_rule_8 = Not (Or f0 f1) in
-         //   let var_for_rule_9 = Not (Not f0) in
-         //   let test_formula = DImplies (Or f1 f2) f0 in
-         //   let out1 = FStar.Printf.sprintf "%s\n" (pretty_print test_formula) in
-            //   print_string out1;
-            //   print_string (pretty_print var_for_rule_3)
-         //   let start_interval = 4 in
-         //   let end_interval = 6 in
-           let l1 = [1;2;3;4;5] in
-           let interv = interval_of_list l1 0 0 in
-           print_string (concat "" (list_int_to_list_string interv))
+let rec print_clause (clause : list int) : string
+   = match clause with
+      | [] -> ""
+      | hd::tl -> 
+           let r = print_clause tl in
+           if r = "" then string_of_int hd
+           else concat " \/ " [string_of_int hd; r]
+
+
+let rec print_cnf_formula (f : list (list int)) : string
+   = match f with
+      | [] -> ""
+      | hd::tl ->
+           let r = print_cnf_formula tl in
+           if r = "" then concat "" ["("; print_clause hd; ")"]
+           else concat " /\ " [concat "" ["("; print_clause hd; ")"]; r]
+
+
+let main = let f0 = Var 0 in
+           let f1 = Var 1 in
+           let f2 = Var 2 in
+           let f3 = Var 3 in 
+
+           let var_for_rule_0 = DImplies f0 f1 in
+           let var_for_rule_1 = Implies f0 f1 in
+           let var_for_rule_2 = Or f0 (And f1 f2) in
+           let var_for_rule_3 = Or (And f1 f2) (DImplies f0 f1) in
+           let var_for_rule_5 = Or f0 (Or f1 f2) in
+           let var_for_rule_6 = And f0 (And f1 f2) in
+           let var_for_rule_7 = Not (And f0 f1) in
+           let var_for_rule_8 = Not (Or f0 f1) in
+           let var_for_rule_9 = Not (Not f0) in
+           let test_formula = DImplies (Or f1 f2) f0 in
+
+           let out1 = FStar.Printf.sprintf "%s\n" (pretty_print test_formula) in
+           print_string out1;
+
+           let cnf = convert_to_cnf test_formula in
+           let out2 = FStar.Printf.sprintf "%s\n" (pretty_print cnf) in
+           print_string out2;
+
+        //    let tseitin_f = tseitin test_formula in
+           let tseitin_f = [[1;2;3]; [0;1]; [2;4]] in
+           let out3 = FStar.Printf.sprintf "%s\n" (print_cnf_formula tseitin_f) in
+           print_string out3
 
