TseitinProofs.fst
@@ -21,8 +21,8 @@ let not_clauses_in_interval (v1:int) (v:int) (n:nat) (start_interval:nat) (end_i
     = ()
 
 
-let prove_same_value_not (f1:formula_t) (rf1 : list (list int)) (v1:int) (n:nat)
-                         (start_interval:nat) (v:int) (end_interval:nat)
+let prove_same_value_not (f1:formula_t) (rf1 : list (list int)) (v1:int) 
+                         (n:nat) (start_interval:nat) (v:int) (end_interval:nat)
                          (rf : list (list int)) 
     : Lemma (requires n <= start_interval /\ start_interval <= v /\
                       valid f1 rf1 v1 n start_interval v /\
@@ -44,9 +44,6 @@ let prove_same_value_not (f1:formula_t) (rf1 : list (list int)) (v1:int) (n:nat)
                            variables_up_to_literal (pos_var_to_lit v) (L.length tau) &&
                            truth_value_literal (pos_var_to_lit v) tau = truth_value (Not f1) tau)
           = variables_up_to_monotone f1 n (L.length tau);
-            // assert (variables_in_interval rf n start_interval end_interval);
-            // variables_in_interval_monotone rf n start_interval start_interval v end_interval;
-            assert (tseitin_same_value f1 rf v1 n start_interval end_interval);
             assert (truth_value_literal (pos_var_to_lit v1) tau = truth_value f1 tau);
             lemma_not_clauses v1 v tau;
             assert (truth_value_literal (pos_var_to_lit v) tau = truth_value (Not f1) tau)
@@ -66,8 +63,8 @@ let or_clauses_in_interval (v1:int) (v2:int) (v:int) (n:nat) (start_interval:nat
 
 let prove_same_value_or (f1:formula_t) (rf1 : list (list int)) (v1:int)
                         (f2:formula_t) (rf2 : list (list int)) (v2:int)
-                        (n:nat) (start_interval:nat) (mid:nat) (end_interval:nat)
-                        (v:int) (rf : list (list int))
+                        (n:nat) (start_interval:nat) (mid:nat) (v:int) (end_interval:nat)
+                        (rf : list (list int))
     : Lemma (requires n <= start_interval /\ start_interval <= mid /\ mid <= v /\
                       valid f1 rf1 v1 n start_interval mid /\
                       tseitin_same_value f1 rf1 v1 n start_interval mid /\
@@ -118,8 +115,8 @@ let and_clauses_in_interval (v1:int) (v2:int) (v:int) (n:nat) (start_interval:na
 
 let prove_same_value_and (f1:formula_t) (rf1 : list (list int)) (v1:int)
                          (f2:formula_t) (rf2 : list (list int)) (v2:int)
-                         (n:nat) (start_interval:nat) (mid:nat) (end_interval:nat)
-                         (v:int) (rf : list (list int))
+                         (n:nat) (start_interval:nat) (mid:nat) (v:int) (end_interval:nat)
+                         (rf : list (list int))
     : Lemma (requires n <= start_interval /\ start_interval <= mid /\ mid <= v /\
                       valid f1 rf1 v1 n start_interval mid /\
                       tseitin_same_value f1 rf1 v1 n start_interval mid /\
@@ -170,8 +167,8 @@ let implies_clauses_in_interval (v1:int) (v2:int) (v:int) (n:nat) (start_interva
 
 let prove_same_value_implies (f1:formula_t) (rf1 : list (list int)) (v1:int)
                              (f2:formula_t) (rf2 : list (list int)) (v2:int)
-                             (n:nat) (start_interval:nat) (mid:nat) (end_interval:nat)
-                             (v:int) (rf : list (list int))
+                             (n:nat) (start_interval:nat) (mid:nat) (v:int)(end_interval:nat)
+                             (rf : list (list int))
     : Lemma (requires n <= start_interval /\ start_interval <= mid /\ mid <= v /\
                       valid f1 rf1 v1 n start_interval mid /\
                       tseitin_same_value f1 rf1 v1 n start_interval mid /\
@@ -204,7 +201,7 @@ let prove_same_value_implies (f1:formula_t) (rf1 : list (list int)) (v1:int)
             variables_up_to_monotone f2 n (L.length tau);
             assert (truth_value_literal (pos_var_to_lit v1) tau = truth_value f1 tau);
             assert (truth_value_literal (pos_var_to_lit v2) tau = truth_value f2 tau);
-            lemma_and_clauses v1 v2 v tau;
+            lemma_implies_clauses v1 v2 v tau;
             assert (truth_value_literal (pos_var_to_lit v) tau = truth_value (Implies f1 f2) tau)
       in
       forall_intro (move_requires aux)
@@ -222,8 +219,8 @@ let dimplies_clauses_in_interval (v1:int) (v2:int) (v:int) (n:nat) (start_interv
 
 let prove_same_value_dimplies (f1:formula_t) (rf1 : list (list int)) (v1:int)
                               (f2:formula_t) (rf2 : list (list int)) (v2:int)
-                              (n:nat) (start_interval:nat) (mid:nat) (end_interval:nat)
-                              (v:int) (rf : list (list int))
+                              (n:nat) (start_interval:nat) (mid:nat) (v:int) (end_interval:nat)
+                              (rf : list (list int))
     : Lemma (requires n <= start_interval /\ start_interval <= mid /\ mid <= v /\
                       valid f1 rf1 v1 n start_interval mid /\
                       tseitin_same_value f1 rf1 v1 n start_interval mid /\
@@ -256,14 +253,15 @@ let prove_same_value_dimplies (f1:formula_t) (rf1 : list (list int)) (v1:int)
             variables_up_to_monotone f2 n (L.length tau);
             assert (truth_value_literal (pos_var_to_lit v1) tau = truth_value f1 tau);
             assert (truth_value_literal (pos_var_to_lit v2) tau = truth_value f2 tau);
-            lemma_and_clauses v1 v2 v tau;
+            lemma_dimplies_clauses v1 v2 v tau;
             assert (truth_value_literal (pos_var_to_lit v) tau = truth_value (DImplies f1 f2) tau)
       in
       forall_intro (move_requires aux)
   
 
-let prove_can_extend_not (f1:formula_t) (rf1 : list (list int)) (v1:int) (n:nat)
-                         (start_interval:nat) (v:int) (end_interval:nat) (rf : list (list int))
+let prove_can_extend_not (f1:formula_t) (rf1 : list (list int)) (v1:int)
+                         (n:nat) (start_interval:nat) (v:int) (end_interval:nat)
+                         (rf : list (list int))
     : Lemma (requires n <= start_interval /\ start_interval <= v /\ v < end_interval /\
                       valid f1 rf1 v1 n start_interval v /\
                       tseitin_can_extend f1 rf1 v1 n start_interval v /\
@@ -310,9 +308,9 @@ let prove_can_extend_not (f1:formula_t) (rf1 : list (list int)) (v1:int) (n:nat)
 
 
 #set-options "--split_queries always"
-let prove_can_extend_or (f1:formula_t) (rf1 : list (list int)) (v1:nat) 
-                        (f2:formula_t) (rf2 : list (list int)) (v2:nat) 
-                        (n:nat) (start_interval:nat) (mid:nat) (v:nat) (end_interval:nat)
+let prove_can_extend_or (f1:formula_t) (rf1 : list (list int)) (v1:int) 
+                        (f2:formula_t) (rf2 : list (list int)) (v2:int) 
+                        (n:nat) (start_interval:nat) (mid:nat) (v:int) (end_interval:nat)
                         (rf :list (list int))
     : Lemma (requires n <= start_interval /\ start_interval <= mid /\ mid <= v /\
                       valid f1 rf1 v1 n start_interval mid /\
@@ -395,9 +393,9 @@ let prove_can_extend_or (f1:formula_t) (rf1 : list (list int)) (v1:nat)
       forall_intro (move_requires aux)
 
 
-let prove_can_extend_and (f1:formula_t) (rf1 : list (list int)) (v1:nat) 
-                         (f2:formula_t) (rf2 : list (list int)) (v2:nat) 
-                         (n:nat) (start_interval:nat) (mid:nat) (v:nat) (end_interval:nat)
+let prove_can_extend_and (f1:formula_t) (rf1 : list (list int)) (v1:int) 
+                         (f2:formula_t) (rf2 : list (list int)) (v2:int) 
+                         (n:nat) (start_interval:nat) (mid:nat) (v:int) (end_interval:nat)
                          (rf :list (list int))
     : Lemma (requires n <= start_interval /\ start_interval <= mid /\ mid <= v /\
                       valid f1 rf1 v1 n start_interval mid /\
@@ -480,9 +478,9 @@ let prove_can_extend_and (f1:formula_t) (rf1 : list (list int)) (v1:nat)
       forall_intro (move_requires aux)
 
 
-let prove_can_extend_implies (f1:formula_t) (rf1 : list (list int)) (v1:nat) 
-                             (f2:formula_t) (rf2 : list (list int)) (v2:nat) 
-                             (n:nat) (start_interval:nat) (mid:nat) (v:nat) (end_interval:nat)
+let prove_can_extend_implies (f1:formula_t) (rf1 : list (list int)) (v1:int) 
+                             (f2:formula_t) (rf2 : list (list int)) (v2:int) 
+                             (n:nat) (start_interval:nat) (mid:nat) (v:int) (end_interval:nat)
                              (rf :list (list int))
     : Lemma (requires n <= start_interval /\ start_interval <= mid /\ mid <= v /\
                       valid f1 rf1 v1 n start_interval mid /\
@@ -563,6 +561,91 @@ let prove_can_extend_implies (f1:formula_t) (rf1 : list (list int)) (v1:nat)
 
             lemma_implies_clauses v1 v2 v tau';
             assert (can_extend tau (Implies f1 f2) rf v n start_interval end_interval)
+      in
+      forall_intro (move_requires aux)
+  
+
+let prove_can_extend_dimplies (f1:formula_t) (rf1 : list (list int)) (v1:int) 
+                              (f2:formula_t) (rf2 : list (list int)) (v2:int) 
+                              (n:nat) (start_interval:nat) (mid:nat) (v:int) (end_interval:nat)
+                              (rf :list (list int))
+    : Lemma (requires n <= start_interval /\ start_interval <= mid /\ mid <= v /\
+                      valid f1 rf1 v1 n start_interval mid /\
+                      tseitin_can_extend f1 rf1 v1 n start_interval mid /\
+                      valid f2 rf2 v2 n mid v /\
+                      tseitin_can_extend f2 rf2 v2 n mid v /\
+                      rf = rf1 @ rf2 @ (dimplies_clauses v1 v2 v) /\
+                      end_interval = v + 1)
+            (ensures valid (DImplies f1 f2) rf v n start_interval end_interval /\
+                     tseitin_can_extend (DImplies f1 f2) rf v n start_interval end_interval)
+    = LP.append_assoc rf1 rf2 (dimplies_clauses v1 v2 v);
+      append_valid_cnf_formulas rf1 rf2;
+      append_valid_cnf_formulas (rf1 @ rf2) (dimplies_clauses v1 v2 v);
+
+      variables_in_interval_monotone rf1 n start_interval start_interval mid end_interval;
+      variables_in_interval_monotone rf2 n mid start_interval v end_interval;
+
+      dimplies_clauses_in_interval v1 v2 v n start_interval mid end_interval;
+      append_variables_in_interval rf1 rf2 n start_interval end_interval;
+      append_variables_in_interval (rf1 @ rf2) (dimplies_clauses v1 v2 v) n start_interval end_interval;assert (valid (DImplies f1 f2) rf v n start_interval end_interval);
+      
+      let aux (tau : list bool) 
+          : Lemma (requires L.length tau = n)
+                  (ensures L.length tau = n /\
+                           can_extend tau (DImplies f1 f2) rf v n start_interval end_interval)
+          = let conditions1 (tau1 : list bool) : Tot bool =
+                is_prefix tau tau1 &&
+                L.length tau1 = mid &&
+                truth_value_cnf_formula rf1 tau1 &&
+                truth_value f1 tau = truth_value_literal (pos_var_to_lit v1) tau1
+            in
+            assume (exists x . conditions1 x);
+            let tau1 = extract_value conditions1 in
+            assert (is_prefix tau tau1);
+            assert (L.length tau1 = mid);
+
+            let conditions2 (tau2 : list bool) : Tot bool =
+                is_prefix tau tau2 &&
+                L.length tau2 = v &&
+                truth_value_cnf_formula rf2 tau2 &&
+                truth_value f2 tau = truth_value_literal (pos_var_to_lit v2) tau2
+            in
+            assume (exists x . conditions2 x);
+            let tau2 = extract_value conditions2 in
+            assert (is_prefix tau tau2);
+            assert (L.length tau2 = v);
+
+
+            let tau' = combine tau tau1 tau2 n start_interval mid v (truth_value (DImplies f1 f2) tau) in
+            assert (L.length tau' = v + 1);
+
+            // assert (interval_of_list tau' 0 n = interval_of_list tau 0 n);
+            assert (interval_of_list tau' start_interval mid = interval_of_list tau1 start_interval mid);
+            assert (interval_of_list tau' mid v = interval_of_list tau2 mid v);
+            assert (L.index tau' v = truth_value (DImplies f1 f2) tau);
+
+            assert (truth_value_literal (pos_var_to_lit v) tau' = truth_value (DImplies f1 f2) tau);
+            assert (truth_value_literal (neg_var_to_lit v) tau' = not (truth_value (DImplies f1 f2) tau));
+
+            is_prefix_then_is_interval tau tau1;
+            transfer_truth_value rf1 tau1 tau' n start_interval mid;
+            is_prefix_then_is_interval tau tau2;
+            transfer_truth_value rf2 tau2 tau' n mid v;
+
+            transfer_truth_value_lit (pos_var_to_lit v1) tau1 tau' n start_interval mid;
+            // assert (truth_value_literal (pos_var_to_lit v1) tau' = truth_value f1 tau);
+            transfer_truth_value_lit (neg_var_to_lit v1) tau1 tau' n start_interval mid;
+            // assert (truth_value_literal (neg_var_to_lit v1) tau' = not (truth_value f1 tau));
+            
+            transfer_truth_value_lit (pos_var_to_lit v2) tau2 tau' n mid v;
+            // assert (truth_value_literal (pos_var_to_lit v2) tau' = truth_value f2 tau);
+            transfer_truth_value_lit (neg_var_to_lit v2) tau2 tau' n mid v;
+            // assert (truth_value_literal (neg_var_to_lit v2) tau' = not (truth_value f1 tau));
+
+            // assert (truth_value (DImplies f1 f2) tau = (truth_value f1 tau <==> truth_value f2 tau));
+
+            lemma_dimplies_clauses v1 v2 v tau';
+            assert (can_extend tau (DImplies f1 f2) rf v n start_interval end_interval)
       in
       forall_intro (move_requires aux)
 #reset-options
