LemmasForClauses.AndClauses.fst
@@ -1,0 +1,175 @@
+module LemmasForClauses.AndClauses
+
+open FStar.List.Tot
+module L = FStar.List.Tot.Base
+module LP = FStar.List.Tot.Properties
+open FStar.Classical
+open FormulaT
+open CnfFormula
+open TseitinCore
+
+
+
+let and_clauses (v1:int {valid_variable v1}) 
+                (v2:int {valid_variable v2}) 
+                (v:int {valid_variable v}) 
+    : r : list (list int) {valid_cnf_formula r}
+    = [[neg_var_to_lit v; pos_var_to_lit v1];
+       [neg_var_to_lit v; pos_var_to_lit v2];
+       [neg_var_to_lit v1; neg_var_to_lit v2; pos_var_to_lit v]]
+
+
+let and_clauses_up_to (v1:int) (v2:int) (v:int) (n:nat)
+    : Lemma (requires valid_variable v1 && valid_variable v2 && valid_variable v &&
+                      n > v1 && n > v2 && n > v)
+            (ensures variables_up_to_cnf_formula (and_clauses v1 v2 v) n)
+    = ()
+
+
+let lemma_and_clauses (v1:int) (v2:int) (v:int) (tau : list bool)
+    : Lemma (requires valid_variable v1 && valid_variable v2 && valid_variable v &&
+                      L.length tau > v1 && L.length tau > v2 && L.length tau > v)
+            (ensures variables_up_to_cnf_formula (and_clauses v1 v2 v) (L.length tau) /\
+                     truth_value_cnf_formula (and_clauses v1 v2 v) tau <==>
+                        ((truth_value_literal (pos_var_to_lit v1) tau && 
+                        truth_value_literal (pos_var_to_lit v2) tau) <==>
+                        truth_value_literal (pos_var_to_lit v) tau))
+    = and_clauses_up_to v1 v2 v (L.length tau)
+
+
+let and_clauses_in_interval (v1:int) (v2:int) (v:int) (n:nat) (start_interval:nat) (mid:nat) (end_interval:nat)
+    : Lemma (requires n <= start_interval && start_interval <= mid && mid <= v &&
+                      valid_variable v1 && valid_variable v2 && valid_variable v &&
+                      variable_in_interval v1 n start_interval mid &&
+                      variable_in_interval v2 n mid v &&
+                      end_interval = v + 1)
+            (ensures variables_in_interval (and_clauses v1 v2 v) n start_interval end_interval)
+    = ()
+
+
+let prove_same_value_and (f1:formula_t) (rf1 : list (list int)) (v1:int)
+                         (f2:formula_t) (rf2 : list (list int)) (v2:int)
+                         (n:nat) (start_interval:nat) (mid:nat) (v:int) (end_interval:nat)
+                         (rf : list (list int))
+    : Lemma (requires n <= start_interval /\ start_interval <= mid /\ mid <= v /\
+                      valid f1 rf1 v1 n start_interval mid /\
+                      tseitin_same_value f1 rf1 v1 n start_interval mid /\
+                      valid f2 rf2 v2 n mid v /\
+                      tseitin_same_value f2 rf2 v2 n mid v /\
+                      rf = rf1 @ rf2 @ (and_clauses v1 v2 v) /\
+                      end_interval = v + 1)
+            (ensures valid (And f1 f2) rf v n start_interval end_interval /\
+                     tseitin_same_value (And f1 f2) rf v n start_interval end_interval)
+    = LP.append_assoc rf1 rf2 (and_clauses v1 v2 v);
+      append_valid_cnf_formulas rf1 rf2;
+      append_valid_cnf_formulas (rf1 @ rf2) (and_clauses v1 v2 v);
+
+      variables_in_interval_monotone rf1 n start_interval start_interval mid end_interval;
+      variables_in_interval_monotone rf2 n mid start_interval v end_interval;
+
+      and_clauses_in_interval v1 v2 v n start_interval mid end_interval;
+      append_variables_in_interval rf1 rf2 n start_interval end_interval;
+      append_variables_in_interval (rf1 @ rf2) (and_clauses v1 v2 v) n start_interval end_interval;
+
+      assert (valid (And f1 f2) rf v n start_interval end_interval);
+
+      let aux (tau : list bool) 
+          : Lemma (requires L.length tau >= end_interval /\
+                            variables_up_to_cnf_formula rf (L.length tau) /\
+                            truth_value_cnf_formula rf tau)
+                  (ensures variables_up_to (And f1 f2) (L.length tau) &&
+                           variables_up_to_literal (pos_var_to_lit v) (L.length tau) &&truth_value_literal (pos_var_to_lit v) tau = truth_value (And f1 f2) tau)
+          = assert (variables_up_to_cnf_formula rf (L.length tau));
+            variables_up_to_monotone f1 n (L.length tau);
+            variables_up_to_monotone f2 n (L.length tau);
+            assert (truth_value_literal (pos_var_to_lit v1) tau = truth_value f1 tau);
+            assert (truth_value_literal (pos_var_to_lit v2) tau = truth_value f2 tau);
+            lemma_and_clauses v1 v2 v tau;
+            assert (truth_value_literal (pos_var_to_lit v) tau = truth_value (And f1 f2) tau)
+      in
+      forall_intro (move_requires aux)
+
+
+let prove_can_extend_and (f1:formula_t) (rf1 : list (list int)) (v1:int) 
+                         (f2:formula_t) (rf2 : list (list int)) (v2:int) 
+                         (n:nat) (start_interval:nat) (mid:nat) (v:int) (end_interval:nat)
+                         (rf :list (list int))
+    : Lemma (requires n <= start_interval /\ start_interval <= mid /\ mid <= v /\
+                      valid f1 rf1 v1 n start_interval mid /\
+                      tseitin_can_extend f1 rf1 v1 n start_interval mid /\
+                      valid f2 rf2 v2 n mid v /\
+                      tseitin_can_extend f2 rf2 v2 n mid v /\
+                      rf = rf1 @ rf2 @ (and_clauses v1 v2 v) /\
+                      end_interval = v + 1)
+            (ensures valid (And f1 f2) rf v n start_interval end_interval /\
+                     tseitin_can_extend (And f1 f2) rf v n start_interval end_interval)
+    = LP.append_assoc rf1 rf2 (and_clauses v1 v2 v);
+      append_valid_cnf_formulas rf1 rf2;
+      append_valid_cnf_formulas (rf1 @ rf2) (and_clauses v1 v2 v);
+
+      variables_in_interval_monotone rf1 n start_interval start_interval mid end_interval;
+      variables_in_interval_monotone rf2 n mid start_interval v end_interval;
+
+      and_clauses_in_interval v1 v2 v n start_interval mid end_interval;
+      append_variables_in_interval rf1 rf2 n start_interval end_interval;
+      append_variables_in_interval (rf1 @ rf2) (and_clauses v1 v2 v) n start_interval end_interval;
+      assert (valid (And f1 f2) rf v n start_interval end_interval)
+      
+      // let aux (tau : list bool)
+      //     : Lemma (requires L.length tau = n)
+      //             (ensures L.length tau = n /\
+      //                      can_extend tau (And f1 f2) rf v n start_interval end_interval)
+      //     = let conditions1 (tau1 : list bool) : Tot bool =
+      //           is_prefix tau tau1 &&
+      //           L.length tau1 = mid &&
+      //           truth_value_cnf_formula rf1 tau1 &&
+      //           truth_value f1 tau = truth_value_literal (pos_var_to_lit v1) tau1
+      //       in
+      //       assume (exists x . conditions1 x);
+      //       let tau1 = extract_value conditions1 in
+      //       assert (is_prefix tau tau1);
+      //       assert (L.length tau1 = mid);
+
+
+      //       let conditions2 (tau2 : list bool) : Tot bool =
+      //           is_prefix tau tau2 &&
+      //           L.length tau2 = v &&
+      //           truth_value_cnf_formula rf2 tau2 &&
+      //           truth_value f2 tau = truth_value_literal (pos_var_to_lit v2) tau2
+      //       in
+      //       assume (exists x . conditions2 x);
+      //       let tau2 = extract_value conditions2 in
+      //       assert (is_prefix tau tau2);
+      //       assert (L.length tau2 = v);
+
+
+      //       let tau' = combine tau tau1 tau2 n start_interval mid v (truth_value (And f1 f2) tau) in
+      //       assert (L.length tau' = v + 1);
+
+      //       // assert (interval_of_list tau' 0 n = interval_of_list tau 0 n);
+      //       assert (interval_of_list tau' start_interval mid = interval_of_list tau1 start_interval mid);
+      //       assert (interval_of_list tau' mid v = interval_of_list tau2 mid v);
+      //       assert (L.index tau' v = truth_value (And f1 f2) tau);
+
+      //       assert (truth_value_literal (pos_var_to_lit v) tau' = truth_value (And f1 f2) tau);
+      //       assert (truth_value_literal (neg_var_to_lit v) tau' = not (truth_value (And f1 f2) tau));
+
+      //       is_prefix_then_is_interval tau tau1;
+      //       transfer_truth_value rf1 tau1 tau' n start_interval mid;
+      //       is_prefix_then_is_interval tau tau2;
+      //       transfer_truth_value rf2 tau2 tau' n mid v;
+
+      //       transfer_truth_value_lit (pos_var_to_lit v1) tau1 tau' n start_interval mid;
+      //       // assert (truth_value_literal (pos_var_to_lit v1) tau' = truth_value f1 tau);
+      //       transfer_truth_value_lit (neg_var_to_lit v1) tau1 tau' n start_interval mid;
+      //       // assert (truth_value_literal (neg_var_to_lit v1) tau' = not (truth_value f1 tau));
+            
+      //       transfer_truth_value_lit (pos_var_to_lit v2) tau2 tau' n mid v;
+      //       // assert (truth_value_literal (pos_var_to_lit v2) tau' = truth_value f2 tau);
+      //       transfer_truth_value_lit (neg_var_to_lit v2) tau2 tau' n mid v;
+      //       // assert (truth_value_literal (neg_var_to_lit v2) tau' = not (truth_value f1 tau));
+
+      //       lemma_and_clauses v1 v2 v tau';
+      //       assert (can_extend tau (And f1 f2) rf v n start_interval end_interval)
+      // in
+      // forall_intro (move_requires aux)
