LemmasForClauses.NotClauses.fst
@@ -1,0 +1,117 @@
+module LemmasForClauses.NotClauses
+
+open FStar.List.Tot
+module L = FStar.List.Tot.Base
+open FStar.Classical
+// open Utils
+open FormulaT
+open CnfFormula
+open TseitinCore
+
+
+
+let not_clauses (v1:int {valid_variable v1})
+                (v:int {valid_variable v})
+    : r : list (list int) {valid_cnf_formula r}
+    = [[neg_var_to_lit v; neg_var_to_lit v1];
+       [pos_var_to_lit v1; pos_var_to_lit v]]
+
+
+let not_clauses_up_to (v1:int) (v:int) (n:nat)
+    : Lemma (requires valid_variable v1 && valid_variable v &&
+                      n > v1 && n > v)
+            (ensures variables_up_to_cnf_formula (not_clauses v1 v) n)
+    = ()
+
+
+let lemma_not_clauses (v1:int) (v:int) (tau : list bool)
+    : Lemma (requires valid_variable v1 && valid_variable v && L.length tau > v && L.length tau > v1)
+            (ensures variables_up_to_cnf_formula (not_clauses v1 v) (L.length tau) /\
+                     truth_value_cnf_formula (not_clauses v1 v) tau <==> 
+                       ((not (truth_value_literal (pos_var_to_lit v1) tau)) <==> 
+                       truth_value_literal (pos_var_to_lit v) tau))
+    = not_clauses_up_to v1 v (L.length tau)
+
+
+let not_clauses_in_interval (v1:int) (v:int) (n:nat) (start_interval:nat) (end_interval:nat)
+    : Lemma (requires n <= start_interval /\ start_interval <= v &&
+                      valid_variable v1 && valid_variable v &&
+                      variable_in_interval v1 n start_interval v &&
+                      end_interval = v + 1)
+            (ensures variables_in_interval (not_clauses v1 v) n start_interval end_interval)
+    = ()
+
+
+let prove_same_value_not (f1:formula_t) (rf1 : list (list int)) (v1:int) (n:nat)
+                         (start_interval:nat) (v:int) (end_interval:nat)
+                         (rf : list (list int)) 
+    : Lemma (requires n <= start_interval /\ start_interval <= v /\
+                      valid f1 rf1 v1 n start_interval v /\
+                      tseitin_same_value f1 rf1 v1 n start_interval v /\
+                      rf = rf1 @ (not_clauses v1 v) /\
+                      end_interval = v + 1)
+            (ensures valid (Not f1) rf v n start_interval end_interval /\
+                     tseitin_same_value (Not f1) rf v n start_interval end_interval)
+    = append_valid_cnf_formulas rf1 (not_clauses v1 v);
+      variables_in_interval_monotone rf1 n start_interval start_interval v end_interval;
+      not_clauses_in_interval v1 v n start_interval end_interval;
+      append_variables_in_interval rf1 (not_clauses v1 v) n start_interval end_interval;
+      assert (valid (Not f1) rf v n start_interval end_interval);
+
+      let aux (tau : list bool) 
+          : Lemma (requires L.length tau >= end_interval &&
+                            truth_value_cnf_formula rf tau)
+                  (ensures variables_up_to (Not f1) (L.length tau) &&
+                           variables_up_to_literal (pos_var_to_lit v) (L.length tau) &&
+                           truth_value_literal (pos_var_to_lit v) tau = truth_value (Not f1) tau)
+          = variables_up_to_monotone f1 n (L.length tau);
+            assert (truth_value_literal (pos_var_to_lit v1) tau = truth_value f1 tau);
+            lemma_not_clauses v1 v tau;
+            assert (truth_value_literal (pos_var_to_lit v) tau = truth_value (Not f1) tau)
+      in
+      forall_intro (move_requires aux)
+
+
+let prove_can_extend_not (f1:formula_t) (rf1 : list (list int)) (v1:int) (n:nat)
+                         (start_interval:nat) (v:int) (end_interval:nat) (rf : list (list int))
+    : Lemma (requires n <= start_interval /\ start_interval <= v /\ v < end_interval /\
+                      valid f1 rf1 v1 n start_interval v /\
+                      tseitin_can_extend f1 rf1 v1 n start_interval v /\
+                      rf = rf1 @ (not_clauses v1 v) /\
+                      end_interval = v + 1)
+            (ensures valid (Not f1) rf v n start_interval end_interval /\
+                     tseitin_can_extend (Not f1) rf v n start_interval end_interval)
+    = append_valid_cnf_formulas rf1 (not_clauses v1 v);
+      variables_in_interval_monotone rf1 n start_interval start_interval v end_interval;
+      not_clauses_in_interval v1 v n start_interval end_interval;
+      append_variables_in_interval rf1 (not_clauses v1 v) n start_interval end_interval;
+      assert (valid (Not f1) rf v n start_interval end_interval)
+
+    //   let aux (tau : list bool) 
+    //       : Lemma (requires L.length tau = n)
+    //               (ensures L.length tau = n /\
+    //                        can_extend tau (Not f1) rf v n start_interval end_interval)
+    //       = assert (can_extend tau f1 rf1 v1 n start_interval v);
+    //         assert (valid_literal (pos_var_to_lit v1));
+            
+    //         let conditions (tau1 : list bool) =
+    //             is_prefix tau tau1 &&
+    //             L.length tau1 = v &&
+    //             truth_value_cnf_formula rf1 tau1 &&
+    //             truth_value f1 tau = truth_value_literal (pos_var_to_lit v1) tau1
+    //         in
+    //         assume (exists x . conditions x);
+    //         let tau1 = extract_value conditions in
+
+    //         negate_literal v1 tau1;
+
+    //         let tau' = combine1 tau tau1 n start_interval v (truth_value (Not f1) tau) in
+    //         is_prefix_then_is_interval tau tau1;
+    //         transfer_truth_value rf1 tau1 tau' n start_interval v
+
+            // transfer_truth_value_lit (pos_var_to_lit v1) tau1 tau' n start_interval v;
+            // transfer_truth_value_lit (neg_var_to_lit v1) tau1 tau' n start_interval v
+
+            //lemma_not_clauses v1 v tau'
+    //   in
+    //   forall_intro (move_requires aux) 
