LemmasForClauses.fst
@@ -1,0 +1,7 @@
+module LemmasForClauses
+
+include LemmasForClauses.NotClauses
+include LemmasForClauses.OrClauses
+include LemmasForClauses.AndClauses
+include LemmasForClauses.ImpliesClauses
+include LemmasForClauses.DImpliesClauses
