Makefile
@@ -2,97 +2,52 @@ include ./Makefile.include
 
 include $(FSTAR_ULIB)/ml/Makefile.include
 
-# OUT_DIR   = out
-# CACHE_DIR = cache
-# ROOTS     = Main.fst
+OUT_DIR   = out
+CACHE_DIR = cache
+ROOTS     = Main.fst
 
-# FSTAR_FLAGS = $(OTHERFLAGS) --cmi --odir $(OUT_DIR) --cache_dir $(CACHE_DIR) \
-#   --cache_checked_modules --already_cached 'Prims FStar'
+FSTAR_FLAGS = $(OTHERFLAGS) --cmi --odir $(OUT_DIR) --cache_dir $(CACHE_DIR) \
+  --cache_checked_modules --already_cached 'Prims FStar'
 
-# FSTAR = $(FSTAR_HOME)/bin/fstar.exe $(FSTAR_FLAGS)
+FSTAR = $(FSTAR_HOME)/bin/fstar.exe $(FSTAR_FLAGS)
 
-# .PHONY: all main clean
+.PHONY: all main clean
 
-# all:
-# 	rm -f .depend && $(MAKE) .depend
-# 	+$(MAKE) main
+all:
+	rm -f .depend && $(MAKE) .depend
+	+$(MAKE) main
 
-# # 1. Extract .ml files
-# # - generate the F* dependency graph of $(ROOTS) with `fstar --dep full`
-# # - verify every F* file in parallel to generate .checked files
-# # - extract each .checked file into a .ml file in parallel
-# .depend:
-# 	$(FSTAR) --dep full $(ROOTS) --extract '* -Prims -FStar' > $@
+# 1. Extract .ml files
+# - generate the F* dependency graph of $(ROOTS) with `fstar --dep full`
+# - verify every F* file in parallel to generate .checked files
+# - extract each .checked file into a .ml file in parallel
+.depend:
+	$(FSTAR) --dep full $(ROOTS) --extract '* -Prims -FStar' > $@
 
-# include .depend
+include .depend
 
-# $(CACHE_DIR)/%.checked: | .depend
-# 	$(FSTAR) $< $(ENABLE_HINTS) --hint_file $(HINT_DIR)/$(notdir $<).hints && \
-# 	touch $@
+$(CACHE_DIR)/%.checked: | .depend
+	$(FSTAR) $< $(ENABLE_HINTS) --hint_file $(HINT_DIR)/$(notdir $<).hints && \
+	touch $@
 
-# # 2. Compile all .ml files to .cmx and link them to get an executable
-# $(OUT_DIR):
-# 	mkdir -p $@
+# 2. Compile all .ml files to .cmx and link them to get an executable
+$(OUT_DIR):
+	mkdir -p $@
 
-# $(OUT_DIR)/%.ml: | .depend
-# 	$(FSTAR) --codegen OCaml \
-# 	  --extract_module $(basename $(notdir $(subst .checked,,$<))) \
-# 	  $(notdir $(subst .checked,,$<)) && \
-# 	touch $@
+$(OUT_DIR)/%.ml: | .depend
+	$(FSTAR) --codegen OCaml \
+	  --extract_module $(basename $(notdir $(subst .checked,,$<))) \
+	  $(notdir $(subst .checked,,$<)) && \
+	touch $@
 
-# %.cmx:
-# 	$(OCAMLOPT) -I $(OUT_DIR) -c $< -o $@
+%.cmx:
+	$(OCAMLOPT) -I $(OUT_DIR) -c $< -o $@
 
-# $(OUT_DIR)/main.exe: $(subst .ml,.cmx,$(ALL_ML_FILES)) | $(OUT_DIR)
-# 	$(OCAMLOPT) -I $(OUT_DIR) -o $(OUT_DIR)/main.exe $(subst .ml,.cmx,$(ALL_ML_FILES))
+$(OUT_DIR)/main.exe: $(subst .ml,.cmx,$(ALL_ML_FILES)) | $(OUT_DIR)
+	$(OCAMLOPT) -I $(OUT_DIR) -o $(OUT_DIR)/main.exe $(subst .ml,.cmx,$(ALL_ML_FILES))
 
-# main: $(OUT_DIR)/main.exe
-# 	$(OUT_DIR)/main.exe
+main: $(OUT_DIR)/main.exe
+	$(OUT_DIR)/main.exe
 
-# clean:
-# 	rm -rf $(OUT_DIR) $(CACHE_DIR)
-
-
-
-
-
-
-cnf: out ./Cnf.fst
-	$(FSTAR) $(FSTAR_DEFAULT_ARGS) --odir out --codegen OCaml --extract 'Cnf' ./Cnf.fst --record_hints 
-	$(OCAMLOPT) out/Cnf.ml -o cnf.exe
-	./cnf.exe
-
-utils: out ./Utils.fst
-	$(FSTAR) $(FSTAR_DEFAULT_ARGS) --odir out --codegen OCaml --extract 'Utils' ./Utils.fst --record_hints
-	$(OCAMLOPT) out/Utils.ml -o utils.exe
-	./utils.exe
-
-formula: out ./FormulaT.fst
-	$(FSTAR) $(FSTAR_DEFAULT_ARGS) --odir out --codegen OCaml --extract 'FormulaT' ./FormulaT.fst --record_hints
-	$(OCAMLOPT) out/FormulaT.ml -o formula.exe
-	./formula.exe
-
-cnfformula: out ./CnfFormula.fst
-	$(FSTAR) $(FSTAR_DEFAULT_ARGS) --odir out --codegen OCaml --extract 'CnfFormula' ./CnfFormula.fst --record_hints
-	$(OCAMLOPT) out/CnfFormula.ml -o cnfformula.exe
-	./cnfformula.exe
-
-tseitincore: out ./TseitinCore.fst
-	$(FSTAR) $(FSTAR_DEFAULT_ARGS) --odir out --codegen OCaml --extract 'TseitinCore' ./TseitinCore.fst --record_hints
-	$(OCAMLOPT) out/TseitinCore.ml -o tseitincore.exe
-	./tseitincore.exe
-
-tseitin: out ./Tseitin.fst
-	$(FSTAR) $(FSTAR_DEFAULT_ARGS) --odir out --codegen OCaml --extract 'Tseitin' ./Tseitin.fst --record_hints
-	$(OCAMLOPT) out/Tseitin.ml -o tseitin.exe
-	./tseitin.exe
-
-tseitinproofs: out ./TseitinProofs.fst
-	$(FSTAR) $(FSTAR_DEFAULT_ARGS) --odir out --codegen OCaml --extract 'TseitinProofs' ./TseitinProofs.fst --record_hints
-	$(OCAMLOPT) out/TseitinProofs.ml -o tseitinproofs.exe
-	./tseitinproofs.exe
-
-main: out ./Main.fst
-	$(FSTAR) $(FSTAR_DEFAULT_ARGS) --odir out --codegen OCaml --extract 'Main' ./Main.fst --record_hints
-	$(OCAMLOPT) out/Main.ml -o main.exe
-	./main.exe
+clean:
+	rm -rf $(OUT_DIR) $(CACHE_DIR)
